<?xml version="1.0"?>
<rdf:RDF xmlns="http://purl.obolibrary.org/obo/bfo-core.owl#"
     xml:base="http://purl.obolibrary.org/obo/bfo-core.owl"
     xmlns:dc="http://purl.org/dc/elements/1.1/"
     xmlns:obo="http://purl.obolibrary.org/obo/"
     xmlns:owl="http://www.w3.org/2002/07/owl#"
     xmlns:rdf="http://www.w3.org/1999/02/22-rdf-syntax-ns#"
     xmlns:xml="http://www.w3.org/XML/1998/namespace"
     xmlns:xsd="http://www.w3.org/2001/XMLSchema#"
     xmlns:rdfs="http://www.w3.org/2000/01/rdf-schema#"
     xmlns:skos="http://www.w3.org/2004/02/skos/core#">
    <owl:Ontology rdf:about="http://purl.obolibrary.org/obo/bfo-core.owl">
        <owl:versionIRI rdf:resource="http://purl.obolibrary.org/obo/1.0.0/bfo-core.owl"/>
        <dc:contributor>Alan Ruttenberg</dc:contributor>
        <dc:contributor>Albert Goldfain</dc:contributor>
        <dc:contributor>Barry Smith</dc:contributor>
        <dc:contributor>Bill Duncan</dc:contributor>
        <dc:contributor>Bjoern Peters</dc:contributor>
        <dc:contributor>Chris Mungall</dc:contributor>
        <dc:contributor>David Osumi-Sutherland</dc:contributor>
        <dc:contributor>Fabian Neuhaus</dc:contributor>
        <dc:contributor>James A. Overton</dc:contributor>
        <dc:contributor>Janna Hastings</dc:contributor>
        <dc:contributor>Jie Zheng</dc:contributor>
        <dc:contributor>John Beverley</dc:contributor>
        <dc:contributor>Jonathan Bona</dc:contributor>
        <dc:contributor>Larry Hunter</dc:contributor>
        <dc:contributor>Leonard Jacuzzo</dc:contributor>
        <dc:contributor>Ludger Jansen</dc:contributor>
        <dc:contributor>Mark Ressler</dc:contributor>
        <dc:contributor>Mathias Brochhausen</dc:contributor>
        <dc:contributor>Mauricio Almeida</dc:contributor>
        <dc:contributor>Melanie Courtot</dc:contributor>
        <dc:contributor>Pierre Grenon</dc:contributor>
        <dc:contributor>Randall Dipert</dc:contributor>
        <dc:contributor>Robert Rovetto</dc:contributor>
        <dc:contributor>Ron Rudnicki</dc:contributor>
        <dc:contributor>Stefan Schulz</dc:contributor>
        <dc:contributor>Thomas Bittner</dc:contributor>
        <dc:contributor>Werner Ceusters</dc:contributor>
        <dc:contributor>Yongqun &quot;Oliver&quot; He</dc:contributor>
        <dc:license rdf:resource="https://creativecommons.org/licenses/by/4.0/"/>
        <rdfs:comment>The most recent version of this file will always be in the GitHub repository https://github.com/bfo-ontology/bfo-2020</rdfs:comment>
        <rdfs:label xml:lang="en">BFO-Core</rdfs:label>
    </owl:Ontology>
    
    <!-- 
    ///////////////////////////////////////////////////////////////////////////////////////
    //
    // Annotation properties
    //
    ///////////////////////////////////////////////////////////////////////////////////////
     -->

    <!-- http://purl.org/dc/elements/1.1/contributor -->

    <owl:AnnotationProperty rdf:about="http://purl.org/dc/elements/1.1/contributor"/>
    


    <!-- http://purl.org/dc/elements/1.1/identifier -->

    <owl:AnnotationProperty rdf:about="http://purl.org/dc/elements/1.1/identifier"/>
    


    <!-- http://purl.org/dc/elements/1.1/license -->

    <owl:AnnotationProperty rdf:about="http://purl.org/dc/elements/1.1/license"/>
    


    <!-- http://www.w3.org/2004/02/skos/core#altLabel -->

    <owl:AnnotationProperty rdf:about="http://www.w3.org/2004/02/skos/core#altLabel"/>
    


    <!-- http://www.w3.org/2004/02/skos/core#definition -->

    <owl:AnnotationProperty rdf:about="http://www.w3.org/2004/02/skos/core#definition"/>
    


    <!-- http://www.w3.org/2004/02/skos/core#example -->

    <owl:AnnotationProperty rdf:about="http://www.w3.org/2004/02/skos/core#example"/>
    


    <!-- http://www.w3.org/2004/02/skos/core#prefLabel -->

    <owl:AnnotationProperty rdf:about="http://www.w3.org/2004/02/skos/core#prefLabel"/>
    


    <!-- http://www.w3.org/2004/02/skos/core#scopeNote -->

    <owl:AnnotationProperty rdf:about="http://www.w3.org/2004/02/skos/core#scopeNote"/>
    


    <!-- 
    ///////////////////////////////////////////////////////////////////////////////////////
    //
    // Object Properties
    //
    ///////////////////////////////////////////////////////////////////////////////////////
     -->

    


    <!-- http://purl.obolibrary.org/obo/BFO_0000054 -->

    <owl:ObjectProperty rdf:about="http://purl.obolibrary.org/obo/BFO_0000054">
        <owl:inverseOf rdf:resource="http://purl.obolibrary.org/obo/BFO_0000055"/>
        <rdfs:domain rdf:resource="http://purl.obolibrary.org/obo/BFO_0000017"/>
        <rdfs:range rdf:resource="http://purl.obolibrary.org/obo/BFO_0000015"/>
        <dc:identifier>206-BFO</dc:identifier>
        <rdfs:label xml:lang="en">has realization</rdfs:label>
        <skos:definition xml:lang="en">b has realization c =Def c realizes b</skos:definition>
        <skos:example xml:lang="en">A disposition to go bald has realization a balding process, a role of student has realization a studying processes, the pumping function of a heart has realization a processes of pumping.</skos:example>
        <skos:prefLabel xml:lang="en">has realization</skos:prefLabel>
    </owl:ObjectProperty>
    


    <!-- http://purl.obolibrary.org/obo/BFO_0000055 -->

    <owl:ObjectProperty rdf:about="http://purl.obolibrary.org/obo/BFO_0000055">
        <rdfs:domain rdf:resource="http://purl.obolibrary.org/obo/BFO_0000015"/>
        <rdfs:range rdf:resource="http://purl.obolibrary.org/obo/BFO_0000017"/>
        <dc:identifier>059-BFO</dc:identifier>
        <rdfs:label xml:lang="en">realizes</rdfs:label>
        <skos:definition xml:lang="en">(Elucidation) realizes is a relation between a process b and a realizable entity c such that inheres in some d and for all t, if b has participant d at t then c exists at t and the type instantiated by b is correlated with the type instantiated by c</skos:definition>
        <skos:example xml:lang="en">A balding process realizes a disposition to go bald, studying realizes a student role, a blood pumping process realizes the pumping function of a heart</skos:example>
        <skos:prefLabel xml:lang="en">realizes</skos:prefLabel>
    </owl:ObjectProperty>
    


    <!-- http://purl.obolibrary.org/obo/BFO_0000062 -->

    <owl:ObjectProperty rdf:about="http://purl.obolibrary.org/obo/BFO_0000062">
        <owl:inverseOf rdf:resource="http://purl.obolibrary.org/obo/BFO_0000063"/>
        <rdf:type rdf:resource="http://www.w3.org/2002/07/owl#TransitiveProperty"/>
        <rdfs:domain rdf:resource="http://purl.obolibrary.org/obo/BFO_0000003"/>
        <rdfs:range rdf:resource="http://purl.obolibrary.org/obo/BFO_0000003"/>
        <dc:identifier>213-BFO</dc:identifier>
        <rdfs:label xml:lang="en">preceded by</rdfs:label>
        <skos:definition xml:lang="en">b preceded by c =Def b precedes c</skos:definition>
        <skos:example xml:lang="en">The temporal region occupied by the second half of the match is preceded by the temporal region occupied by the first half of the match</skos:example>
        <skos:prefLabel xml:lang="en">preceded by</skos:prefLabel>
    </owl:ObjectProperty>
    


    <!-- http://purl.obolibrary.org/obo/BFO_0000063 -->

    <owl:ObjectProperty rdf:about="http://purl.obolibrary.org/obo/BFO_0000063">
        <rdf:type rdf:resource="http://www.w3.org/2002/07/owl#TransitiveProperty"/>
        <rdfs:domain rdf:resource="http://purl.obolibrary.org/obo/BFO_0000003"/>
        <rdfs:range rdf:resource="http://purl.obolibrary.org/obo/BFO_0000003"/>
        <dc:identifier>270-BFO</dc:identifier>
        <rdfs:label xml:lang="en">precedes</rdfs:label>
        <skos:definition xml:lang="en">(Elucidation) precedes is a relation that holds between occurrents o, o&apos; with respective temporal extents t, t&apos;, such that either the last instant of o is before the first instant of o&apos; or the last instant of o is the first instant of o&apos; and neither o nor o&apos; are temporal instants</skos:definition>
        <skos:example xml:lang="en">The temporal region occupied by Mary&apos;s birth precedes the temporal region occupied by Mary&apos;s death</skos:example>
        <skos:prefLabel xml:lang="en">precedes</skos:prefLabel>
        <skos:scopeNote xml:lang="en">Each temporal region is its own temporal extent. The temporal extent of a spatiotemporal region is the temporal region it temporally projects onto. The temporal extent of a process or process boundary that occupies temporal region t is t.</skos:scopeNote>
        <skos:scopeNote xml:lang="en">Precedes defines a strict partial order on occurrents.</skos:scopeNote>
    </owl:ObjectProperty>
    


    <!-- http://purl.obolibrary.org/obo/BFO_0000066 -->

    <owl:ObjectProperty rdf:about="http://purl.obolibrary.org/obo/BFO_0000066">
        <owl:inverseOf rdf:resource="http://purl.obolibrary.org/obo/BFO_0000183"/>
        <rdfs:domain>
            <owl:Class>
                <owl:unionOf rdf:parseType="Collection">
                    <rdf:Description rdf:about="http://purl.obolibrary.org/obo/BFO_0000015"/>
                    <rdf:Description rdf:about="http://purl.obolibrary.org/obo/BFO_0000035"/>
                </owl:unionOf>
            </owl:Class>
        </rdfs:domain>
        <rdfs:range>
            <owl:Class>
                <owl:unionOf rdf:parseType="Collection">
                    <rdf:Description rdf:about="http://purl.obolibrary.org/obo/BFO_0000029"/>
                    <rdf:Description rdf:about="http://purl.obolibrary.org/obo/BFO_0000040"/>
                </owl:unionOf>
            </owl:Class>
        </rdfs:range>
        <dc:identifier>143-BFO</dc:identifier>
        <rdfs:label xml:lang="en">occurs in</rdfs:label>
        <skos:definition xml:lang="en">b occurs in c =Def b is a process or a process boundary and c is a material entity or site, and for all t if b exists at t then c exists at t, b occupies a spatiotemporal region r that spatially projects onto spatial region s at t, c occupies spatial region s&apos; at t, and s is continuant part of s&apos; at t</skos:definition>
        <skos:example xml:lang="en">A process of digestion occurs in the interior of an organism, a process of loading artillery rounds into a tank cannon occurs in the interior of the tank</skos:example>
        <skos:prefLabel xml:lang="en">occurs in</skos:prefLabel>
    </owl:ObjectProperty>
    


    <!-- http://purl.obolibrary.org/obo/BFO_0000108 -->

    <owl:ObjectProperty rdf:about="http://purl.obolibrary.org/obo/BFO_0000108">
        <rdfs:domain>
            <owl:Class>
                <owl:unionOf rdf:parseType="Collection">
                    <rdf:Description rdf:about="http://purl.obolibrary.org/obo/BFO_0000002"/>
                    <rdf:Description rdf:about="http://purl.obolibrary.org/obo/BFO_0000003"/>
                </owl:unionOf>
            </owl:Class>
        </rdfs:domain>
        <rdfs:range rdf:resource="http://purl.obolibrary.org/obo/BFO_0000008"/>
        <dc:identifier>118-BFO</dc:identifier>
        <rdfs:label xml:lang="en">exists at</rdfs:label>
        <skos:definition xml:lang="en">(Elucidation) exists at is a relation between a particular and some temporal region at which the particular exists</skos:definition>
        <skos:example xml:lang="en">First World War exists at 1914-1916, Mexico exists at January 1, 2000</skos:example>
        <skos:prefLabel xml:lang="en">exists at</skos:prefLabel>
    </owl:ObjectProperty>
    


    <!-- http://purl.obolibrary.org/obo/BFO_0000117 -->

    <owl:ObjectProperty rdf:about="http://purl.obolibrary.org/obo/BFO_0000117">
        <owl:inverseOf rdf:resource="http://purl.obolibrary.org/obo/BFO_0000132"/>
        <rdf:type rdf:resource="http://www.w3.org/2002/07/owl#TransitiveProperty"/>
        <rdfs:domain rdf:resource="http://purl.obolibrary.org/obo/BFO_0000003"/>
        <rdfs:range rdf:resource="http://purl.obolibrary.org/obo/BFO_0000003"/>
        <dc:identifier>202-BFO</dc:identifier>
        <rdfs:label xml:lang="en">has occurrent part</rdfs:label>
        <skos:definition xml:lang="en">(Elucidation) has occurrent part is a relation between an occurrent c and occurrent b when c is a part of b</skos:definition>
        <skos:example xml:lang="en">Mary&apos;s life has occurrent part Mary&apos;s 5th birthday</skos:example>
        <skos:prefLabel xml:lang="en">has occurrent part</skos:prefLabel>
    </owl:ObjectProperty>
    


    <!-- http://purl.obolibrary.org/obo/BFO_0000118 -->

    <owl:ObjectProperty rdf:about="http://purl.obolibrary.org/obo/BFO_0000118">
        <rdfs:subPropertyOf rdf:resource="http://purl.obolibrary.org/obo/BFO_0000117"/>
        <owl:inverseOf rdf:resource="http://purl.obolibrary.org/obo/BFO_0000138"/>
        <rdf:type rdf:resource="http://www.w3.org/2002/07/owl#TransitiveProperty"/>
        <rdfs:domain rdf:resource="http://purl.obolibrary.org/obo/BFO_0000003"/>
        <rdfs:range rdf:resource="http://purl.obolibrary.org/obo/BFO_0000003"/>
        <dc:identifier>154-BFO</dc:identifier>
        <rdfs:label xml:lang="en">has proper occurrent part</rdfs:label>
        <skos:definition xml:lang="en">b has proper occurrent part c =Def b has occurrent part c and b and c are not identical</skos:definition>
        <skos:example xml:lang="en">As for has occurrent part</skos:example>
        <skos:prefLabel xml:lang="en">has proper occurrent part</skos:prefLabel>
    </owl:ObjectProperty>
    


    <!-- http://purl.obolibrary.org/obo/BFO_0000121 -->

    <owl:ObjectProperty rdf:about="http://purl.obolibrary.org/obo/BFO_0000121">
        <rdfs:subPropertyOf rdf:resource="http://purl.obolibrary.org/obo/BFO_0000117"/>
        <owl:inverseOf rdf:resource="http://purl.obolibrary.org/obo/BFO_0000139"/>
        <rdf:type rdf:resource="http://www.w3.org/2002/07/owl#TransitiveProperty"/>
        <rdfs:domain rdf:resource="http://purl.obolibrary.org/obo/BFO_0000003"/>
        <rdfs:range rdf:resource="http://purl.obolibrary.org/obo/BFO_0000003"/>
        <dc:identifier>211-BFO</dc:identifier>
        <rdfs:label xml:lang="en">has temporal part</rdfs:label>
        <skos:definition xml:lang="en">b has temporal part c =Def c temporal part of b</skos:definition>
        <skos:example xml:lang="en">Your life has temporal part the first year of your life</skos:example>
        <skos:prefLabel xml:lang="en">has temporal part</skos:prefLabel>
    </owl:ObjectProperty>
    


    <!-- http://purl.obolibrary.org/obo/BFO_0000132 -->

    <owl:ObjectProperty rdf:about="http://purl.obolibrary.org/obo/BFO_0000132">
        <rdf:type rdf:resource="http://www.w3.org/2002/07/owl#TransitiveProperty"/>
        <rdfs:domain rdf:resource="http://purl.obolibrary.org/obo/BFO_0000003"/>
        <rdfs:range rdf:resource="http://purl.obolibrary.org/obo/BFO_0000003"/>
        <dc:identifier>003-BFO</dc:identifier>
        <rdfs:label xml:lang="en">occurrent part of</rdfs:label>
        <skos:definition xml:lang="en">(Elucidation) b occurrent part of c =Def c has occurrent part b</skos:definition>
        <skos:example xml:lang="en">Mary&apos;s 5th birthday is an occurrent part of Mary&apos;s life, the first set of the tennis match is an occurrent part of the tennis match</skos:example>
        <skos:prefLabel xml:lang="en">occurrent part of</skos:prefLabel>
    </owl:ObjectProperty>
    


    <!-- http://purl.obolibrary.org/obo/BFO_0000136 -->

    <owl:ObjectProperty rdf:about="http://purl.obolibrary.org/obo/BFO_0000136">
        <rdfs:subPropertyOf rdf:resource="http://purl.obolibrary.org/obo/BFO_0000139"/>
        <owl:inverseOf rdf:resource="http://purl.obolibrary.org/obo/BFO_0000181"/>
        <rdfs:domain rdf:resource="http://purl.obolibrary.org/obo/BFO_0000003"/>
        <rdfs:range rdf:resource="http://purl.obolibrary.org/obo/BFO_0000003"/>
        <dc:identifier>116-BFO</dc:identifier>
        <rdfs:label xml:lang="en">proper temporal part of</rdfs:label>
        <skos:definition xml:lang="en">b proper temporal part of c =Def b temporal part of c and b and c are not identical</skos:definition>
        <skos:example xml:lang="en">As for temporal part of</skos:example>
        <skos:prefLabel xml:lang="en">proper temporal part of</skos:prefLabel>
    </owl:ObjectProperty>
    


    <!-- http://purl.obolibrary.org/obo/BFO_0000138 -->

    <owl:ObjectProperty rdf:about="http://purl.obolibrary.org/obo/BFO_0000138">
        <rdfs:subPropertyOf rdf:resource="http://purl.obolibrary.org/obo/BFO_0000132"/>
        <rdf:type rdf:resource="http://www.w3.org/2002/07/owl#TransitiveProperty"/>
        <rdfs:domain rdf:resource="http://purl.obolibrary.org/obo/BFO_0000003"/>
        <rdfs:range rdf:resource="http://purl.obolibrary.org/obo/BFO_0000003"/>
        <dc:identifier>005-BFO</dc:identifier>
        <rdfs:label xml:lang="en">proper occurrent part of</rdfs:label>
        <skos:definition xml:lang="en">b proper occurrent part of c =Def b occurrent part of c &amp; b and c are not identical</skos:definition>
        <skos:example xml:lang="en">As for occurrent part of</skos:example>
        <skos:prefLabel xml:lang="en">proper occurrent part of</skos:prefLabel>
    </owl:ObjectProperty>
    


    <!-- http://purl.obolibrary.org/obo/BFO_0000139 -->

    <owl:ObjectProperty rdf:about="http://purl.obolibrary.org/obo/BFO_0000139">
        <rdfs:subPropertyOf rdf:resource="http://purl.obolibrary.org/obo/BFO_0000132"/>
        <rdf:type rdf:resource="http://www.w3.org/2002/07/owl#TransitiveProperty"/>
        <rdfs:domain rdf:resource="http://purl.obolibrary.org/obo/BFO_0000003"/>
        <rdfs:range rdf:resource="http://purl.obolibrary.org/obo/BFO_0000003"/>
        <dc:identifier>078-BFO</dc:identifier>
        <rdfs:label xml:lang="en">temporal part of</rdfs:label>
        <skos:definition xml:lang="en">b temporal part of c =Def b occurrent part of c and either b and c are temporal regions or b and c are spatiotemporal regions, b temporally projects onto an occurrent part of the temporal region that c temporally projects onto or b and c are processes or process boundaries and b occupies a temporal region that is an occurrent part of the temporal region that c occupies</skos:definition>
        <skos:example xml:lang="en">Your heart beating from 4pm to 5pm today is a temporal part of the process of your heart beating, the 4th year of your life is a temporal part of your life, as is the process boundary which separates the 3rd and 4th years of your life, the first quarter of a game of football is a temporal part of the whole game</skos:example>
        <skos:prefLabel xml:lang="en">temporal part of</skos:prefLabel>
    </owl:ObjectProperty>
    


    <!-- http://purl.obolibrary.org/obo/BFO_0000153 -->

    <owl:ObjectProperty rdf:about="http://purl.obolibrary.org/obo/BFO_0000153">
        <rdf:type rdf:resource="http://www.w3.org/2002/07/owl#FunctionalProperty"/>
        <rdfs:domain rdf:resource="http://purl.obolibrary.org/obo/BFO_0000011"/>
        <rdfs:range rdf:resource="http://purl.obolibrary.org/obo/BFO_0000008"/>
        <dc:identifier>080-BFO</dc:identifier>
        <rdfs:label xml:lang="en">temporally projects onto</rdfs:label>
        <skos:definition xml:lang="en">(Elucidation) temporally projects onto is a relation between a spatiotemporal region and some temporal region which is its temporal extent</skos:definition>
        <skos:example xml:lang="en">The world line of a particle temporally projects onto the temporal region extending from the beginning to the end of the existence of the particle</skos:example>
        <skos:prefLabel xml:lang="en">temporally projects onto</skos:prefLabel>
    </owl:ObjectProperty>
    


    <!-- http://purl.obolibrary.org/obo/BFO_0000181 -->

    <owl:ObjectProperty rdf:about="http://purl.obolibrary.org/obo/BFO_0000181">
        <rdfs:subPropertyOf rdf:resource="http://purl.obolibrary.org/obo/BFO_0000121"/>
        <rdfs:domain rdf:resource="http://purl.obolibrary.org/obo/BFO_0000003"/>
        <rdfs:range rdf:resource="http://purl.obolibrary.org/obo/BFO_0000003"/>
        <dc:identifier>212-BFO</dc:identifier>
        <rdfs:label xml:lang="en">has proper temporal part</rdfs:label>
        <skos:definition xml:lang="en">b has proper temporal part c =Def c proper temporal part of b</skos:definition>
        <skos:example xml:lang="en">As for has temporal part</skos:example>
        <skos:prefLabel xml:lang="en">has proper temporal part</skos:prefLabel>
    </owl:ObjectProperty>
    


    <!-- http://purl.obolibrary.org/obo/BFO_0000183 -->

    <owl:ObjectProperty rdf:about="http://purl.obolibrary.org/obo/BFO_0000183">
        <rdfs:domain>
            <owl:Class>
                <owl:unionOf rdf:parseType="Collection">
                    <rdf:Description rdf:about="http://purl.obolibrary.org/obo/BFO_0000029"/>
                    <rdf:Description rdf:about="http://purl.obolibrary.org/obo/BFO_0000040"/>
                </owl:unionOf>
            </owl:Class>
        </rdfs:domain>
        <rdfs:range>
            <owl:Class>
                <owl:unionOf rdf:parseType="Collection">
                    <rdf:Description rdf:about="http://purl.obolibrary.org/obo/BFO_0000015"/>
                    <rdf:Description rdf:about="http://purl.obolibrary.org/obo/BFO_0000035"/>
                </owl:unionOf>
            </owl:Class>
        </rdfs:range>
        <dc:identifier>267-BFO</dc:identifier>
        <rdfs:label xml:lang="en">environs</rdfs:label>
        <skos:definition xml:lang="en">b environs c =Def c occurs in b</skos:definition>
        <skos:example xml:lang="en">A mouth environs a process of mastication, a city environs traffic</skos:example>
        <skos:prefLabel xml:lang="en">environs</skos:prefLabel>
    </owl:ObjectProperty>
    


    <!-- http://purl.obolibrary.org/obo/BFO_0000184 -->

    <owl:ObjectProperty rdf:about="http://purl.obolibrary.org/obo/BFO_0000184">
        <owl:inverseOf rdf:resource="http://purl.obolibrary.org/obo/BFO_0000185"/>
        <rdf:type rdf:resource="http://www.w3.org/2002/07/owl#FunctionalProperty"/>
        <rdf:type rdf:resource="http://www.w3.org/2002/07/owl#InverseFunctionalProperty"/>
        <rdfs:domain rdf:resource="http://purl.obolibrary.org/obo/BFO_0000182"/>
        <rdfs:range rdf:resource="http://purl.obolibrary.org/obo/BFO_0000040"/>
        <dc:identifier>144-BFO</dc:identifier>
        <rdfs:label xml:lang="en">history of</rdfs:label>
        <skos:definition xml:lang="en">(Elucidation) history of is a relation between a history b and a material entity c when b is the unique history of c</skos:definition>
        <skos:example xml:lang="en">This life is the history of this organism</skos:example>
        <skos:prefLabel xml:lang="en">history of</skos:prefLabel>
    </owl:ObjectProperty>
    


    <!-- http://purl.obolibrary.org/obo/BFO_0000185 -->

    <owl:ObjectProperty rdf:about="http://purl.obolibrary.org/obo/BFO_0000185">
        <rdfs:domain rdf:resource="http://purl.obolibrary.org/obo/BFO_0000040"/>
        <rdfs:range rdf:resource="http://purl.obolibrary.org/obo/BFO_0000182"/>
        <dc:identifier>145-BFO</dc:identifier>
        <rdfs:label xml:lang="en">has history</rdfs:label>
        <skos:definition xml:lang="en">b has history c =Def c history of b</skos:definition>
        <skos:example xml:lang="en">This organism has history this life</skos:example>
        <skos:prefLabel xml:lang="en">has history</skos:prefLabel>
    </owl:ObjectProperty>
    


    <!-- http://purl.obolibrary.org/obo/BFO_0000194 -->

    <owl:ObjectProperty rdf:about="http://purl.obolibrary.org/obo/BFO_0000194">
        <owl:inverseOf rdf:resource="http://purl.obolibrary.org/obo/BFO_0000195"/>
        <rdfs:domain>
            <owl:Class>
                <owl:unionOf rdf:parseType="Collection">
                    <rdf:Description rdf:about="http://purl.obolibrary.org/obo/BFO_0000020"/>
                    <owl:Class>
                        <owl:intersectionOf rdf:parseType="Collection">
                            <rdf:Description rdf:about="http://purl.obolibrary.org/obo/BFO_0000004"/>
                            <owl:Class>
                                <owl:complementOf rdf:resource="http://purl.obolibrary.org/obo/BFO_0000006"/>
                            </owl:Class>
                        </owl:intersectionOf>
                    </owl:Class>
                </owl:unionOf>
            </owl:Class>
        </rdfs:domain>
        <rdfs:range rdf:resource="http://purl.obolibrary.org/obo/BFO_0000020"/>
        <dc:identifier>260-BFO</dc:identifier>
        <rdfs:label xml:lang="en">specifically depended on by</rdfs:label>
        <skos:altLabel xml:lang="en">s-depended on by</skos:altLabel>
        <skos:definition xml:lang="en">b s-depended on by c =Def c specifically depends on b</skos:definition>
        <skos:example xml:lang="en">A tomato is s-depended on a redness quality</skos:example>
        <skos:prefLabel xml:lang="en">specifically depended on by</skos:prefLabel>
    </owl:ObjectProperty>
    


    <!-- http://purl.obolibrary.org/obo/BFO_0000195 -->

    <owl:ObjectProperty rdf:about="http://purl.obolibrary.org/obo/BFO_0000195">
        <rdfs:domain rdf:resource="http://purl.obolibrary.org/obo/BFO_0000020"/>
        <rdfs:range>
            <owl:Class>
                <owl:unionOf rdf:parseType="Collection">
                    <rdf:Description rdf:about="http://purl.obolibrary.org/obo/BFO_0000020"/>
                    <owl:Class>
                        <owl:intersectionOf rdf:parseType="Collection">
                            <rdf:Description rdf:about="http://purl.obolibrary.org/obo/BFO_0000004"/>
                            <owl:Class>
                                <owl:complementOf rdf:resource="http://purl.obolibrary.org/obo/BFO_0000006"/>
                            </owl:Class>
                        </owl:intersectionOf>
                    </owl:Class>
                </owl:unionOf>
            </owl:Class>
        </rdfs:range>
        <dc:identifier>012-BFO</dc:identifier>
        <rdfs:label xml:lang="en">specifically depends on</rdfs:label>
        <skos:altLabel xml:lang="en">s-depends on</skos:altLabel>
        <skos:definition xml:lang="en">(Elucidation) specifically depends is a relation between a specifically dependent continuant b and and a specifically dependent continuant or independent continuant that is not a spatial region c, such that b and c do not share common parts, b is of a nature such that at all times t it cannot exist at t unless c exists at t, and b is not a boundary of c</skos:definition>
        <skos:example xml:lang="en">A shape s-depends on the shaped object, hue, saturation and brightness of a colour sample s-depend on each other</skos:example>
        <skos:prefLabel xml:lang="en">specifically depends on</skos:prefLabel>
        <skos:scopeNote xml:lang="en">The analogue of s-dependence for occurrents is has participant.</skos:scopeNote>
    </owl:ObjectProperty>
    


    <!-- http://purl.obolibrary.org/obo/BFO_0000196 -->

    <owl:ObjectProperty rdf:about="http://purl.obolibrary.org/obo/BFO_0000196">
        <rdfs:subPropertyOf rdf:resource="http://purl.obolibrary.org/obo/BFO_0000194"/>
        <owl:inverseOf rdf:resource="http://purl.obolibrary.org/obo/BFO_0000197"/>
        <rdfs:domain>
            <owl:Class>
                <owl:intersectionOf rdf:parseType="Collection">
                    <rdf:Description rdf:about="http://purl.obolibrary.org/obo/BFO_0000004"/>
                    <owl:Class>
                        <owl:complementOf rdf:resource="http://purl.obolibrary.org/obo/BFO_0000006"/>
                    </owl:Class>
                </owl:intersectionOf>
            </owl:Class>
        </rdfs:domain>
        <rdfs:range rdf:resource="http://purl.obolibrary.org/obo/BFO_0000020"/>
        <dc:identifier>053-BFO</dc:identifier>
        <rdfs:label xml:lang="en">bearer of</rdfs:label>
        <skos:definition xml:lang="en">b bearer of c =Def c inheres in b</skos:definition>
        <skos:example xml:lang="en">A patch of ink is the bearer of a colour quality, an organism is the bearer of a temperature quality</skos:example>
        <skos:prefLabel xml:lang="en">bearer of</skos:prefLabel>
    </owl:ObjectProperty>
    


    <!-- http://purl.obolibrary.org/obo/BFO_0000197 -->

    <owl:ObjectProperty rdf:about="http://purl.obolibrary.org/obo/BFO_0000197">
        <rdfs:subPropertyOf rdf:resource="http://purl.obolibrary.org/obo/BFO_0000195"/>
        <rdfs:domain rdf:resource="http://purl.obolibrary.org/obo/BFO_0000020"/>
        <rdfs:range>
            <owl:Class>
                <owl:intersectionOf rdf:parseType="Collection">
                    <rdf:Description rdf:about="http://purl.obolibrary.org/obo/BFO_0000004"/>
                    <owl:Class>
                        <owl:complementOf rdf:resource="http://purl.obolibrary.org/obo/BFO_0000006"/>
                    </owl:Class>
                </owl:intersectionOf>
            </owl:Class>
        </rdfs:range>
        <dc:identifier>051-BFO</dc:identifier>
        <rdfs:label xml:lang="en">inheres in</rdfs:label>
        <skos:definition xml:lang="en">b inheres in c =Def b is a specifically dependent continuant and c is an independent continuant that is not a spatial region and b s-depends on c</skos:definition>
        <skos:example xml:lang="en">A shape inheres in a shaped object, a mass inheres in a material entity</skos:example>
        <skos:prefLabel xml:lang="en">inheres in</skos:prefLabel>
    </owl:ObjectProperty>
    


    <!-- http://purl.obolibrary.org/obo/BFO_0000199 -->

    <owl:ObjectProperty rdf:about="http://purl.obolibrary.org/obo/BFO_0000199">
        <rdf:type rdf:resource="http://www.w3.org/2002/07/owl#FunctionalProperty"/>
        <rdfs:domain>
            <owl:Class>
                <owl:unionOf rdf:parseType="Collection">
                    <rdf:Description rdf:about="http://purl.obolibrary.org/obo/BFO_0000015"/>
                    <rdf:Description rdf:about="http://purl.obolibrary.org/obo/BFO_0000035"/>
                </owl:unionOf>
            </owl:Class>
        </rdfs:domain>
        <rdfs:range rdf:resource="http://purl.obolibrary.org/obo/BFO_0000008"/>
        <dc:identifier>132-BFO</dc:identifier>
        <rdfs:label xml:lang="en">occupies temporal region</rdfs:label>
        <skos:definition xml:lang="en">process or process boundary p occupies temporal region t =Def the spatiotemporal region occupied by p temporally projects onto t</skos:definition>
        <skos:example xml:lang="en">The Second World War occupies the temporal region September 1, 1939 - September 2, 1945</skos:example>
        <skos:prefLabel xml:lang="en">occupies temporal region</skos:prefLabel>
    </owl:ObjectProperty>
    


    <!-- http://purl.obolibrary.org/obo/BFO_0000200 -->

    <owl:ObjectProperty rdf:about="http://purl.obolibrary.org/obo/BFO_0000200">
        <rdf:type rdf:resource="http://www.w3.org/2002/07/owl#FunctionalProperty"/>
        <rdfs:domain>
            <owl:Class>
                <owl:unionOf rdf:parseType="Collection">
                    <rdf:Description rdf:about="http://purl.obolibrary.org/obo/BFO_0000015"/>
                    <rdf:Description rdf:about="http://purl.obolibrary.org/obo/BFO_0000035"/>
                </owl:unionOf>
            </owl:Class>
        </rdfs:domain>
        <rdfs:range rdf:resource="http://purl.obolibrary.org/obo/BFO_0000011"/>
        <dc:identifier>082-BFO</dc:identifier>
        <rdfs:label xml:lang="en">occupies spatiotemporal region</rdfs:label>
        <skos:definition xml:lang="en">(Elucidation) occupies spatiotemporal region is a relation between a process or process boundary and the spatiotemporal region which is its spatiotemporal extent</skos:definition>
        <skos:example xml:lang="en">A particle emitted by a nuclear reactor occupies the spatiotemporal region which is its trajectory</skos:example>
        <skos:prefLabel xml:lang="en">occupies spatiotemporal region</skos:prefLabel>
    </owl:ObjectProperty>
    


    <!-- http://purl.obolibrary.org/obo/BFO_0000221 -->

    <owl:ObjectProperty rdf:about="http://purl.obolibrary.org/obo/BFO_0000221">
        <owl:inverseOf rdf:resource="http://purl.obolibrary.org/obo/BFO_0000222"/>
        <rdfs:domain rdf:resource="http://purl.obolibrary.org/obo/BFO_0000203"/>
        <rdfs:range rdf:resource="http://purl.obolibrary.org/obo/BFO_0000008"/>
        <dc:identifier>268-BFO</dc:identifier>
        <rdfs:label xml:lang="en">first instant of</rdfs:label>
        <skos:definition xml:lang="en">temporal instant t first instant of temporal region t&apos; =Def t precedes all temporal parts of t&apos; other than t</skos:definition>
        <skos:example xml:lang="en">An hour starting at midnight yesterday has first instant midnight yesterday</skos:example>
        <skos:prefLabel xml:lang="en">first instant of</skos:prefLabel>
    </owl:ObjectProperty>
    


    <!-- http://purl.obolibrary.org/obo/BFO_0000222 -->

    <owl:ObjectProperty rdf:about="http://purl.obolibrary.org/obo/BFO_0000222">
        <rdf:type rdf:resource="http://www.w3.org/2002/07/owl#FunctionalProperty"/>
        <rdfs:domain rdf:resource="http://purl.obolibrary.org/obo/BFO_0000008"/>
        <rdfs:range rdf:resource="http://purl.obolibrary.org/obo/BFO_0000203"/>
        <dc:identifier>261-BFO</dc:identifier>
        <rdfs:label xml:lang="en">has first instant</rdfs:label>
        <skos:definition xml:lang="en">t has first instant t&apos; =Def t&apos; first instant of t</skos:definition>
        <skos:example xml:lang="en">The first hour of a year has first instant midnight on December 31</skos:example>
        <skos:prefLabel xml:lang="en">has first instant</skos:prefLabel>
    </owl:ObjectProperty>
    


    <!-- http://purl.obolibrary.org/obo/BFO_0000223 -->

    <owl:ObjectProperty rdf:about="http://purl.obolibrary.org/obo/BFO_0000223">
        <owl:inverseOf rdf:resource="http://purl.obolibrary.org/obo/BFO_0000224"/>
        <rdfs:domain rdf:resource="http://purl.obolibrary.org/obo/BFO_0000203"/>
        <rdfs:range rdf:resource="http://purl.obolibrary.org/obo/BFO_0000008"/>
        <dc:identifier>269-BFO</dc:identifier>
        <rdfs:label xml:lang="en">last instant of</rdfs:label>
        <skos:definition xml:lang="en">temporal instant t last instant of temporal region t&apos; =Def all temporal parts of t&apos; other than t precede t</skos:definition>
        <skos:example xml:lang="en">Last midnight is the last instant of yesterday</skos:example>
        <skos:prefLabel xml:lang="en">last instant of</skos:prefLabel>
    </owl:ObjectProperty>
    


    <!-- http://purl.obolibrary.org/obo/BFO_0000224 -->

    <owl:ObjectProperty rdf:about="http://purl.obolibrary.org/obo/BFO_0000224">
        <rdf:type rdf:resource="http://www.w3.org/2002/07/owl#FunctionalProperty"/>
        <rdfs:domain rdf:resource="http://purl.obolibrary.org/obo/BFO_0000008"/>
        <rdfs:range rdf:resource="http://purl.obolibrary.org/obo/BFO_0000203"/>
        <dc:identifier>215-BFO</dc:identifier>
        <rdfs:label xml:lang="en">has last instant</rdfs:label>
        <skos:definition xml:lang="en">t has last instant t&apos; =Def t&apos; last instant of t</skos:definition>
        <skos:example xml:lang="en">The last hour of a year has last instant midnight December 31</skos:example>
        <skos:prefLabel xml:lang="en">has last instant</skos:prefLabel>
    </owl:ObjectProperty>
    


    <!-- 
    ///////////////////////////////////////////////////////////////////////////////////////
    //
    // Classes
    //
    ///////////////////////////////////////////////////////////////////////////////////////
     -->

    


    <!-- http://purl.obolibrary.org/obo/BFO_0000001 -->

    <owl:Class rdf:about="http://purl.obolibrary.org/obo/BFO_0000001">
        <dc:identifier>001-BFO</dc:identifier>
        <rdfs:label xml:lang="en">entity</rdfs:label>
        <skos:definition xml:lang="en">(Elucidation) An entity is anything that exists or has existed or will exist</skos:definition>
        <skos:example xml:lang="en">Julius Caesar, the Second World War, your body mass index, Verdi&apos;s Requiem</skos:example>
        <skos:prefLabel xml:lang="en">entity</skos:prefLabel>
    </owl:Class>
    


    <!-- http://purl.obolibrary.org/obo/BFO_0000002 -->

    <owl:Class rdf:about="http://purl.obolibrary.org/obo/BFO_0000002">
        <rdfs:subClassOf rdf:resource="http://purl.obolibrary.org/obo/BFO_0000001"/>
        <owl:disjointWith rdf:resource="http://purl.obolibrary.org/obo/BFO_0000003"/>
        <dc:identifier>008-BFO</dc:identifier>
        <rdfs:label xml:lang="en">continuant</rdfs:label>
        <skos:definition xml:lang="en">(Elucidation) A continuant is an entity that persists, endures, or continues to exist through time while maintaining its identity</skos:definition>
        <skos:example xml:lang="en">A human being, a tennis ball, a cave, a region of space, someone&apos;s temperature</skos:example>
        <skos:prefLabel xml:lang="en">continuant</skos:prefLabel>
    </owl:Class>
    


    <!-- http://purl.obolibrary.org/obo/BFO_0000003 -->

    <owl:Class rdf:about="http://purl.obolibrary.org/obo/BFO_0000003">
        <rdfs:subClassOf rdf:resource="http://purl.obolibrary.org/obo/BFO_0000001"/>
        <dc:identifier>077-BFO</dc:identifier>
        <rdfs:label xml:lang="en">occurrent</rdfs:label>
        <skos:definition xml:lang="en">(Elucidation) An occurrent is an entity that unfolds itself in time, or is the start or end of such an entity, or is a temporal or spatiotemporal region</skos:definition>
        <skos:example xml:lang="en">As for process, history, process boundary, spatiotemporal region, zero-dimensional temporal region, one-dimensional temporal region, temporal interval, temporal instant</skos:example>
        <skos:prefLabel xml:lang="en">occurrent</skos:prefLabel>
    </owl:Class>
    


    <!-- http://purl.obolibrary.org/obo/BFO_0000004 -->

    <owl:Class rdf:about="http://purl.obolibrary.org/obo/BFO_0000004">
        <rdfs:subClassOf rdf:resource="http://purl.obolibrary.org/obo/BFO_0000002"/>
        <dc:identifier>017-BFO</dc:identifier>
        <rdfs:label xml:lang="en">independent continuant</rdfs:label>
        <skos:definition xml:lang="en">b is an independent continuant =Def b is a continuant which is such that there is no c such that b s-depends on c and no c such that b g-depends on c</skos:definition>
        <skos:example xml:lang="en">An atom, a molecule, an organism, a heart, a chair, the bottom right portion of a human torso, a leg, the interior of your mouth, a spatial region, an orchestra</skos:example>
        <skos:prefLabel xml:lang="en">independent continuant</skos:prefLabel>
    </owl:Class>
    


    <!-- http://purl.obolibrary.org/obo/BFO_0000006 -->

    <owl:Class rdf:about="http://purl.obolibrary.org/obo/BFO_0000006">
        <rdfs:subClassOf rdf:resource="http://purl.obolibrary.org/obo/BFO_0000141"/>
        <dc:identifier>035-BFO</dc:identifier>
        <rdfs:label xml:lang="en">spatial region</rdfs:label>
        <skos:definition xml:lang="en">(Elucidation) A spatial region is an immaterial entity that is continuant part of the spatial projection of a portion of spacetime at a given time</skos:definition>
        <skos:example xml:lang="en">As for zero-dimensional spatial region, one-dimensional spatial region, two-dimensional spatial region, three-dimensional spatial region</skos:example>
        <skos:prefLabel xml:lang="en">spatial region</skos:prefLabel>
    </owl:Class>
    


    <!-- http://purl.obolibrary.org/obo/BFO_0000008 -->

    <owl:Class rdf:about="http://purl.obolibrary.org/obo/BFO_0000008">
        <rdfs:subClassOf rdf:resource="http://purl.obolibrary.org/obo/BFO_0000003"/>
        <rdfs:subClassOf>
            <owl:Restriction>
                <owl:onProperty rdf:resource="http://purl.obolibrary.org/obo/BFO_0000132"/>
                <owl:allValuesFrom rdf:resource="http://purl.obolibrary.org/obo/BFO_0000008"/>
            </owl:Restriction>
        </rdfs:subClassOf>
        <rdfs:subClassOf>
            <owl:Restriction>
                <owl:onProperty rdf:resource="http://purl.obolibrary.org/obo/BFO_0000139"/>
                <owl:allValuesFrom rdf:resource="http://purl.obolibrary.org/obo/BFO_0000008"/>
            </owl:Restriction>
        </rdfs:subClassOf>
        <dc:identifier>100-BFO</dc:identifier>
        <rdfs:label xml:lang="en">temporal region</rdfs:label>
        <skos:definition xml:lang="en">(Elucidation) A temporal region is an occurrent over which processes can unfold</skos:definition>
        <skos:example xml:lang="en">As for zero-dimensional temporal region and one-dimensional temporal region</skos:example>
        <skos:prefLabel xml:lang="en">temporal region</skos:prefLabel>
    </owl:Class>
    


    <!-- http://purl.obolibrary.org/obo/BFO_0000009 -->

    <owl:Class rdf:about="http://purl.obolibrary.org/obo/BFO_0000009">
        <rdfs:subClassOf rdf:resource="http://purl.obolibrary.org/obo/BFO_0000006"/>
        <dc:identifier>039-BFO</dc:identifier>
        <rdfs:label xml:lang="en">two-dimensional spatial region</rdfs:label>
        <skos:definition xml:lang="en">(Elucidation) A two-dimensional spatial region is a spatial region that is a whole consisting of a surface together with zero or more surfaces and/or spatial regions of lower dimension as parts</skos:definition>
        <skos:example xml:lang="en">The surface of a sphere-shaped part of space, an infinitely thin plane in space</skos:example>
        <skos:prefLabel xml:lang="en">two-dimensional spatial region</skos:prefLabel>
    </owl:Class>
    


    <!-- http://purl.obolibrary.org/obo/BFO_0000011 -->

    <owl:Class rdf:about="http://purl.obolibrary.org/obo/BFO_0000011">
        <rdfs:subClassOf rdf:resource="http://purl.obolibrary.org/obo/BFO_0000003"/>
        <rdfs:subClassOf>
            <owl:Restriction>
                <owl:onProperty rdf:resource="http://purl.obolibrary.org/obo/BFO_0000132"/>
                <owl:allValuesFrom rdf:resource="http://purl.obolibrary.org/obo/BFO_0000011"/>
            </owl:Restriction>
        </rdfs:subClassOf>
        <rdfs:subClassOf>
            <owl:Restriction>
                <owl:onProperty rdf:resource="http://purl.obolibrary.org/obo/BFO_0000139"/>
                <owl:allValuesFrom rdf:resource="http://purl.obolibrary.org/obo/BFO_0000011"/>
            </owl:Restriction>
        </rdfs:subClassOf>
        <dc:identifier>095-BFO</dc:identifier>
        <rdfs:label xml:lang="en">spatiotemporal region</rdfs:label>
        <skos:definition xml:lang="en">(Elucidation) A spatiotemporal region is an occurrent that is an occurrent part of spacetime</skos:definition>
        <skos:example xml:lang="en">The spatiotemporal region occupied by the development of a cancer tumour, the spatiotemporal region occupied by an orbiting satellite</skos:example>
        <skos:prefLabel xml:lang="en">spatiotemporal region</skos:prefLabel>
        <skos:scopeNote xml:lang="en">&apos;Spacetime&apos; here refers to the maximal instance of the universal spatiotemporal region.</skos:scopeNote>
    </owl:Class>
    


    <!-- http://purl.obolibrary.org/obo/BFO_0000015 -->

    <owl:Class rdf:about="http://purl.obolibrary.org/obo/BFO_0000015">
        <rdfs:subClassOf rdf:resource="http://purl.obolibrary.org/obo/BFO_0000003"/>
        <rdfs:subClassOf>
            <owl:Restriction>
                <owl:onProperty rdf:resource="http://purl.obolibrary.org/obo/BFO_0000117"/>
                <owl:allValuesFrom>
                    <owl:Class>
                        <owl:unionOf rdf:parseType="Collection">
                            <rdf:Description rdf:about="http://purl.obolibrary.org/obo/BFO_0000015"/>
                            <rdf:Description rdf:about="http://purl.obolibrary.org/obo/BFO_0000035"/>
                        </owl:unionOf>
                    </owl:Class>
                </owl:allValuesFrom>
            </owl:Restriction>
        </rdfs:subClassOf>
        <rdfs:subClassOf>
            <owl:Restriction>
                <owl:onProperty rdf:resource="http://purl.obolibrary.org/obo/BFO_0000132"/>
                <owl:allValuesFrom rdf:resource="http://purl.obolibrary.org/obo/BFO_0000015"/>
            </owl:Restriction>
        </rdfs:subClassOf>
        <rdfs:subClassOf>
            <owl:Restriction>
                <owl:onProperty rdf:resource="http://purl.obolibrary.org/obo/BFO_0000139"/>
                <owl:allValuesFrom rdf:resource="http://purl.obolibrary.org/obo/BFO_0000015"/>
            </owl:Restriction>
        </rdfs:subClassOf>
        <dc:identifier>083-BFO</dc:identifier>
        <rdfs:label xml:lang="en">process</rdfs:label>
        <skos:definition xml:lang="en">(Elucidation) A process p is an occurrent that has some temporal proper part and for some time t, p has some material entity as participant at t</skos:definition>
        <skos:example xml:lang="en">An act of selling, the life of an organism, a process of sleeping, a process of cell-division, a beating of the heart, a process of meiosis, the taxiing of an aircraft, the programming of a computer</skos:example>
        <skos:prefLabel xml:lang="en">process</skos:prefLabel>
    </owl:Class>
    


    <!-- http://purl.obolibrary.org/obo/BFO_0000016 -->

    <owl:Class rdf:about="http://purl.obolibrary.org/obo/BFO_0000016">
        <rdfs:subClassOf rdf:resource="http://purl.obolibrary.org/obo/BFO_0000017"/>
        <owl:disjointWith rdf:resource="http://purl.obolibrary.org/obo/BFO_0000023"/>
        <dc:identifier>062-BFO</dc:identifier>
        <rdfs:label xml:lang="en">disposition</rdfs:label>
        <skos:altLabel xml:lang="en">internally-grounded realizable entity</skos:altLabel>
        <skos:definition xml:lang="en">(Elucidation) A disposition b is a realizable entity and such that if b ceases to exist, then its bearer is physically changed, and b&apos;s realization occurs when and because this bearer is in some special physical circumstances, and this realization occurs in virtue of the bearer&apos;s physical make-up</skos:definition>
        <skos:example xml:lang="en">An atom of element X has the disposition to decay to an atom of element Y, the cell wall is disposed to transport cellular material through endocytosis and exocytosis, certain people have a disposition to develop colon cancer, children are innately disposed to categorize objects in certain ways</skos:example>
        <skos:prefLabel xml:lang="en">disposition</skos:prefLabel>
    </owl:Class>
    


    <!-- http://purl.obolibrary.org/obo/BFO_0000017 -->

    <owl:Class rdf:about="http://purl.obolibrary.org/obo/BFO_0000017">
        <rdfs:subClassOf rdf:resource="http://purl.obolibrary.org/obo/BFO_0000020"/>
        <owl:disjointWith rdf:resource="http://purl.obolibrary.org/obo/BFO_0000019"/>
        <dc:identifier>058-BFO</dc:identifier>
        <rdfs:label xml:lang="en">realizable entity</rdfs:label>
        <skos:definition xml:lang="en">(Elucidation) A realizable entity b is a specifically dependent continuant that inheres in some independent continuant which is not a spatial region and is of a type some instances of which are realized in processes of a correlated type</skos:definition>
        <skos:example xml:lang="en">The role of being a doctor, the role of this boundary to delineate where Utah and Colorado meet, the function of your reproductive organs, the disposition of your blood to coagulate, the disposition of this piece of metal to conduct electricity</skos:example>
        <skos:prefLabel xml:lang="en">realizable entity</skos:prefLabel>
    </owl:Class>
    


    <!-- http://purl.obolibrary.org/obo/BFO_0000018 -->

    <owl:Class rdf:about="http://purl.obolibrary.org/obo/BFO_0000018">
        <rdfs:subClassOf rdf:resource="http://purl.obolibrary.org/obo/BFO_0000006"/>
        <dc:identifier>037-BFO</dc:identifier>
        <rdfs:label xml:lang="en">zero-dimensional spatial region</rdfs:label>
        <skos:definition xml:lang="en">(Elucidation) A zero-dimensional spatial region is a spatial region that is one or a collection of more than one spatially disjoint points in space</skos:definition>
        <skos:example xml:lang="en">The spatial region occupied at some time instant by the North Pole</skos:example>
        <skos:prefLabel xml:lang="en">zero-dimensional spatial region</skos:prefLabel>
    </owl:Class>
    


    <!-- http://purl.obolibrary.org/obo/BFO_0000019 -->

    <owl:Class rdf:about="http://purl.obolibrary.org/obo/BFO_0000019">
        <rdfs:subClassOf rdf:resource="http://purl.obolibrary.org/obo/BFO_0000020"/>
        <dc:identifier>055-BFO</dc:identifier>
        <rdfs:label xml:lang="en">quality</rdfs:label>
        <skos:definition xml:lang="en">(Elucidation) A quality is a specifically dependent continuant that, in contrast to roles and dispositions, does not require any further process in order to be realized</skos:definition>
        <skos:example xml:lang="en">The colour of a tomato, the ambient temperature of this portion of air, the length of the circumference of your waist, the shape of your nose, the shape of your nostril, the mass of this piece of gold</skos:example>
        <skos:prefLabel xml:lang="en">quality</skos:prefLabel>
    </owl:Class>
    


    <!-- http://purl.obolibrary.org/obo/BFO_0000020 -->

    <owl:Class rdf:about="http://purl.obolibrary.org/obo/BFO_0000020">
        <rdfs:subClassOf rdf:resource="http://purl.obolibrary.org/obo/BFO_0000002"/>
        <dc:identifier>050-BFO</dc:identifier>
        <rdfs:label xml:lang="en">specifically dependent continuant</rdfs:label>
        <skos:definition xml:lang="en">b is a specifically dependent continuant =Def b is a continuant and there is some independent continuant c which is not a spatial region and which is such that b s-depends on c</skos:definition>
        <skos:example xml:lang="en">(with one bearer) The mass of this tomato, the pink colour of a medium rare piece of grilled filet mignon at its centre, the smell of this portion of mozzarella, the disposition of this fish to decay, the role of being a doctor, the function of this heart to pump blood, the shape of this hole
(with multiple bearers:) John&apos;s love for Mary, the ownership relation between John and this statue, the relation of authority between John and his subordinates</skos:example>
        <skos:prefLabel xml:lang="en">specifically dependent continuant</skos:prefLabel>
        <skos:scopeNote xml:lang="en">On the multiple bearers case, see relational quality.</skos:scopeNote>
    </owl:Class>
    


    <!-- http://purl.obolibrary.org/obo/BFO_0000023 -->

    <owl:Class rdf:about="http://purl.obolibrary.org/obo/BFO_0000023">
        <rdfs:subClassOf rdf:resource="http://purl.obolibrary.org/obo/BFO_0000017"/>
        <dc:identifier>061-BFO</dc:identifier>
        <rdfs:label xml:lang="en">role</rdfs:label>
        <skos:altLabel xml:lang="en">externally-grounded realizable entity</skos:altLabel>
        <skos:definition xml:lang="en">(Elucidation) A role b is a realizable entity and exists because there is some single bearer that is in some special physical, social, or institutional set of circumstances in which this bearer does not have to be, and b is not such that, if it ceases to exist, then the physical make-up of the bearer is thereby changed</skos:definition>
        <skos:example xml:lang="en">The priest role, the student role, the role of subject in a clinical trial, the role of a stone in marking a property boundary, the role of a boundary to demarcate two neighbouring administrative territories, the role of a building in serving as a military target</skos:example>
        <skos:prefLabel xml:lang="en">role</skos:prefLabel>
    </owl:Class>
    


    <!-- http://purl.obolibrary.org/obo/BFO_0000024 -->

    <owl:Class rdf:about="http://purl.obolibrary.org/obo/BFO_0000024">
        <rdfs:subClassOf rdf:resource="http://purl.obolibrary.org/obo/BFO_0000040"/>
        <dc:identifier>027-BFO</dc:identifier>
        <rdfs:label xml:lang="en">fiat object part</rdfs:label>
        <skos:definition xml:lang="en">(Elucidation) A fiat object part b is a material entity which is such that for all times t, if b exists at t then there is some object c such that b is a proper continuant part of c at t and b is demarcated from the remainder of c by one or more fiat surfaces</skos:definition>
        <skos:example xml:lang="en">The upper and lower lobes of the left lung, the dorsal and ventral surfaces of the body, the Western hemisphere of the Earth, the regional parts of an intact human body</skos:example>
        <skos:prefLabel xml:lang="en">fiat object part</skos:prefLabel>
    </owl:Class>
    


    <!-- http://purl.obolibrary.org/obo/BFO_0000026 -->

    <owl:Class rdf:about="http://purl.obolibrary.org/obo/BFO_0000026">
        <rdfs:subClassOf rdf:resource="http://purl.obolibrary.org/obo/BFO_0000006"/>
        <dc:identifier>038-BFO</dc:identifier>
        <rdfs:label xml:lang="en">one-dimensional spatial region</rdfs:label>
        <skos:definition xml:lang="en">(Elucidation) A one-dimensional spatial region is a spatial region that is a whole consisting of a line together with zero or more lines and/or points as parts</skos:definition>
        <skos:example xml:lang="en">An edge of a cube-shaped portion of space, a line connecting two points, two parallel lines extended in space</skos:example>
        <skos:prefLabel xml:lang="en">one-dimensional spatial region</skos:prefLabel>
    </owl:Class>
    


    <!-- http://purl.obolibrary.org/obo/BFO_0000027 -->

    <owl:Class rdf:about="http://purl.obolibrary.org/obo/BFO_0000027">
        <rdfs:subClassOf rdf:resource="http://purl.obolibrary.org/obo/BFO_0000040"/>
        <dc:identifier>025-BFO</dc:identifier>
        <rdfs:label xml:lang="en">object aggregate</rdfs:label>
        <skos:definition xml:lang="en">(Elucidation) An object aggregate is a material entity consisting exactly of a plurality (≥1) of objects as member parts which together form a unit</skos:definition>
        <skos:example xml:lang="en">The aggregate of the musicians in a symphony orchestra and their instruments, the aggregate of bearings in a constant velocity axle joint, the nitrogen atoms in the atmosphere, a collection of cells in a blood biobank</skos:example>
        <skos:prefLabel xml:lang="en">object aggregate</skos:prefLabel>
        <skos:scopeNote xml:lang="en">&apos;Exactly&apos; means that there are no parts of the object aggregate other than its member parts.</skos:scopeNote>
        <skos:scopeNote xml:lang="en">The unit can, at certain times, consist of exactly one object, for example, when a wolf litter loses all but one of its pups, but it must at some time have a plurality of member parts.</skos:scopeNote>
    </owl:Class>
    


    <!-- http://purl.obolibrary.org/obo/BFO_0000028 -->

    <owl:Class rdf:about="http://purl.obolibrary.org/obo/BFO_0000028">
        <rdfs:subClassOf rdf:resource="http://purl.obolibrary.org/obo/BFO_0000006"/>
        <dc:identifier>040-BFO</dc:identifier>
        <rdfs:label xml:lang="en">three-dimensional spatial region</rdfs:label>
        <skos:definition xml:lang="en">(Elucidation) A three-dimensional spatial region is a spatial region that is a whole consisting of a spatial volume together with zero or more spatial volumes and/or spatial regions of lower dimension as parts</skos:definition>
        <skos:example xml:lang="en">A cube-shaped region of space, a sphere-shaped region of space, the region of space occupied by all and only the planets in the solar system at some point in time</skos:example>
        <skos:prefLabel xml:lang="en">three-dimensional spatial region</skos:prefLabel>
    </owl:Class>
    


    <!-- http://purl.obolibrary.org/obo/BFO_0000029 -->

    <owl:Class rdf:about="http://purl.obolibrary.org/obo/BFO_0000029">
        <rdfs:subClassOf rdf:resource="http://purl.obolibrary.org/obo/BFO_0000141"/>
        <dc:identifier>034-BFO</dc:identifier>
        <rdfs:label xml:lang="en">site</rdfs:label>
        <skos:definition xml:lang="en">(Elucidation) A site b is an immaterial entity of three dimensions whose boundaries either (1) (partially or wholly) coincide with the boundaries of one or more material entities or (2) have locations determined in relation to some material entity</skos:definition>
        <skos:example xml:lang="en">A hole in a portion of cheese, a rabbit hole, the Grand Canyon, the Piazza San Marco, the kangaroo-joey-containing hole of a kangaroo pouch, your left nostril (a fiat part - the opening - of your left nasal cavity), the lumen of your gut, the hold of a ship, the interior of the trunk of your car, hole in an engineered floor joist, an air traffic control region of type A is determined in terms of elevation above mean sea level of lower and upper boundaries</skos:example>
        <skos:prefLabel xml:lang="en">site</skos:prefLabel>
    </owl:Class>
    


    <!-- http://purl.obolibrary.org/obo/BFO_0000030 -->

    <owl:Class rdf:about="http://purl.obolibrary.org/obo/BFO_0000030">
        <rdfs:subClassOf rdf:resource="http://purl.obolibrary.org/obo/BFO_0000040"/>
        <dc:identifier>024-BFO</dc:identifier>
        <rdfs:label xml:lang="en">object</rdfs:label>
        <skos:definition xml:lang="en">(Elucidation) An object is a material entity which manifests causal unity and is of a type instances of which are maximal relative to the sort of causal unity manifested</skos:definition>
        <skos:example xml:lang="en">An organism, a fish tank, a planet, a laptop, a valve, a block of marble, an ice cube</skos:example>
        <skos:prefLabel xml:lang="en">object</skos:prefLabel>
        <skos:scopeNote xml:lang="en">There are three major types of causal unity: causal unity via physical covering (e.g. interior parts bound by common membrane), causal unity via physical forces (e.g. interior parts bound by ionic or covalent bonds), and causal unity via engineered assembly of components (e.g. dovetail joints, balls and bearings).</skos:scopeNote>
        <skos:scopeNote xml:lang="en">To say that b is &apos;causally unified&apos; is to say that if b has a continuant part c at time t in its interior and c is moved outside the spatial region occupied by b at t, then either b&apos;s other parts move in a coordinated fashion or b is damaged, broken, torn, etc.</skos:scopeNote>
    </owl:Class>
    


    <!-- http://purl.obolibrary.org/obo/BFO_0000031 -->

    <owl:Class rdf:about="http://purl.obolibrary.org/obo/BFO_0000031">
        <rdfs:subClassOf rdf:resource="http://purl.obolibrary.org/obo/BFO_0000002"/>
        <dc:identifier>074-BFO</dc:identifier>
        <rdfs:label xml:lang="en">generically dependent continuant</rdfs:label>
        <skos:altLabel xml:lang="en">g-dependent continuant</skos:altLabel>
        <skos:definition xml:lang="en">(Elucidation) A generically dependent continuant is a continuant that exists in virtue of the fact that there is at least one of what may be multiple copies; it is the content or the pattern that the multiple copies share</skos:definition>
        <skos:example xml:lang="en">The pdf file on your laptop and the pdf file that is a copy thereof on my laptop; the sequence of this protein molecule and the sequence that is a copy thereof in that protein molecule, the content that is shared by a string of dots and dashes written on a page and the transmitted Morse code signal, the content of a sentence, an engineering blueprint</skos:example>
        <skos:prefLabel xml:lang="en">generically dependent continuant</skos:prefLabel>
    </owl:Class>
    


    <!-- http://purl.obolibrary.org/obo/BFO_0000034 -->

    <owl:Class rdf:about="http://purl.obolibrary.org/obo/BFO_0000034">
        <rdfs:subClassOf rdf:resource="http://purl.obolibrary.org/obo/BFO_0000016"/>
        <dc:identifier>064-BFO</dc:identifier>
        <rdfs:label xml:lang="en">function</rdfs:label>
        <skos:definition xml:lang="en">(Elucidation) A function is a disposition that exists in virtue of its bearer&apos;s physical make-up and this physical make-up is something the bearer possesses because it came into being either through evolution (in the case of natural biological entities) or through intentional design (in the case of artefacts), in order to realize processes of a certain sort</skos:definition>
        <skos:example xml:lang="en">The function of a hammer to drive in nails, the function of a heart pacemaker to regulate the beating of a heart through electricity</skos:example>
        <skos:prefLabel xml:lang="en">function</skos:prefLabel>
    </owl:Class>
    


    <!-- http://purl.obolibrary.org/obo/BFO_0000035 -->

    <owl:Class rdf:about="http://purl.obolibrary.org/obo/BFO_0000035">
        <rdfs:subClassOf rdf:resource="http://purl.obolibrary.org/obo/BFO_0000003"/>
        <rdfs:subClassOf>
            <owl:Restriction>
                <owl:onProperty rdf:resource="http://purl.obolibrary.org/obo/BFO_0000117"/>
                <owl:allValuesFrom rdf:resource="http://purl.obolibrary.org/obo/BFO_0000035"/>
            </owl:Restriction>
        </rdfs:subClassOf>
        <rdfs:subClassOf>
            <owl:Restriction>
                <owl:onProperty rdf:resource="http://purl.obolibrary.org/obo/BFO_0000121"/>
                <owl:allValuesFrom rdf:resource="http://purl.obolibrary.org/obo/BFO_0000035"/>
            </owl:Restriction>
        </rdfs:subClassOf>
        <rdfs:subClassOf>
            <owl:Restriction>
                <owl:onProperty rdf:resource="http://purl.obolibrary.org/obo/BFO_0000132"/>
                <owl:allValuesFrom>
                    <owl:Class>
                        <owl:unionOf rdf:parseType="Collection">
                            <rdf:Description rdf:about="http://purl.obolibrary.org/obo/BFO_0000015"/>
                            <rdf:Description rdf:about="http://purl.obolibrary.org/obo/BFO_0000035"/>
                        </owl:unionOf>
                    </owl:Class>
                </owl:allValuesFrom>
            </owl:Restriction>
        </rdfs:subClassOf>
        <rdfs:subClassOf>
            <owl:Restriction>
                <owl:onProperty rdf:resource="http://purl.obolibrary.org/obo/BFO_0000139"/>
                <owl:allValuesFrom>
                    <owl:Class>
                        <owl:unionOf rdf:parseType="Collection">
                            <rdf:Description rdf:about="http://purl.obolibrary.org/obo/BFO_0000015"/>
                            <rdf:Description rdf:about="http://purl.obolibrary.org/obo/BFO_0000035"/>
                        </owl:unionOf>
                    </owl:Class>
                </owl:allValuesFrom>
            </owl:Restriction>
        </rdfs:subClassOf>
        <dc:identifier>084-BFO</dc:identifier>
        <rdfs:label xml:lang="en">process boundary</rdfs:label>
        <skos:definition xml:lang="en">p is a process boundary =Def p is an occurrent, is a temporal part of a process, and p has no proper temporal parts</skos:definition>
        <skos:example xml:lang="en">The boundary between the 2nd and 3rd year of your life</skos:example>
        <skos:prefLabel xml:lang="en">process boundary</skos:prefLabel>
    </owl:Class>
    


    <!-- http://purl.obolibrary.org/obo/BFO_0000038 -->

    <owl:Class rdf:about="http://purl.obolibrary.org/obo/BFO_0000038">
        <rdfs:subClassOf rdf:resource="http://purl.obolibrary.org/obo/BFO_0000008"/>
        <rdfs:subClassOf>
            <owl:Restriction>
                <owl:onProperty rdf:resource="http://purl.obolibrary.org/obo/BFO_0000121"/>
                <owl:allValuesFrom>
                    <owl:Class>
                        <owl:unionOf rdf:parseType="Collection">
                            <rdf:Description rdf:about="http://purl.obolibrary.org/obo/BFO_0000038"/>
                            <rdf:Description rdf:about="http://purl.obolibrary.org/obo/BFO_0000148"/>
                        </owl:unionOf>
                    </owl:Class>
                </owl:allValuesFrom>
            </owl:Restriction>
        </rdfs:subClassOf>
        <rdfs:subClassOf>
            <owl:Restriction>
                <owl:onProperty rdf:resource="http://purl.obolibrary.org/obo/BFO_0000139"/>
                <owl:allValuesFrom rdf:resource="http://purl.obolibrary.org/obo/BFO_0000038"/>
            </owl:Restriction>
        </rdfs:subClassOf>
        <owl:disjointWith rdf:resource="http://purl.obolibrary.org/obo/BFO_0000148"/>
        <dc:identifier>103-BFO</dc:identifier>
        <rdfs:label xml:lang="en">one-dimensional temporal region</rdfs:label>
        <skos:definition xml:lang="en">(Elucidation) A one-dimensional temporal region is a temporal region that is a whole having a temporal interval and zero or more temporal intervals and temporal instants as parts</skos:definition>
        <skos:example xml:lang="en">The temporal region during which a process occurs</skos:example>
        <skos:prefLabel xml:lang="en">one-dimensional temporal region</skos:prefLabel>
    </owl:Class>
    


    <!-- http://purl.obolibrary.org/obo/BFO_0000040 -->

    <owl:Class rdf:about="http://purl.obolibrary.org/obo/BFO_0000040">
        <rdfs:subClassOf rdf:resource="http://purl.obolibrary.org/obo/BFO_0000004"/>
        <owl:disjointWith rdf:resource="http://purl.obolibrary.org/obo/BFO_0000141"/>
        <dc:identifier>019-BFO</dc:identifier>
        <rdfs:label xml:lang="en">material entity</rdfs:label>
        <skos:definition xml:lang="en">(Elucidation) A material entity is an independent continuant that at all times at which it exists has some portion of matter as continuant part</skos:definition>
        <skos:example xml:lang="en">A human being, the undetached arm of a human being, an aggregate of human beings</skos:example>
        <skos:prefLabel xml:lang="en">material entity</skos:prefLabel>
    </owl:Class>
    


    <!-- http://purl.obolibrary.org/obo/BFO_0000140 -->

    <owl:Class rdf:about="http://purl.obolibrary.org/obo/BFO_0000140">
        <rdfs:subClassOf rdf:resource="http://purl.obolibrary.org/obo/BFO_0000141"/>
        <dc:identifier>029-BFO</dc:identifier>
        <rdfs:label xml:lang="en">continuant fiat boundary</rdfs:label>
        <skos:definition xml:lang="en">(Elucidation) A continuant fiat boundary b is an immaterial entity that is of zero, one, or two dimensions, whose location is determined in relation to some material entity, and which is such that there is no time t when b has a spatial region as continuant part at t</skos:definition>
        <skos:example xml:lang="en">As for fiat point, fiat line, and fiat surface</skos:example>
        <skos:prefLabel xml:lang="en">continuant fiat boundary</skos:prefLabel>
    </owl:Class>
    


    <!-- http://purl.obolibrary.org/obo/BFO_0000141 -->

    <owl:Class rdf:about="http://purl.obolibrary.org/obo/BFO_0000141">
        <rdfs:subClassOf rdf:resource="http://purl.obolibrary.org/obo/BFO_0000004"/>
        <dc:identifier>028-BFO</dc:identifier>
        <rdfs:label xml:lang="en">immaterial entity</rdfs:label>
        <skos:definition xml:lang="en">a is an immaterial entity =Def a is an independent continuant which is such that there is no time t when it has a material entity as continuant part at t</skos:definition>
        <skos:example xml:lang="en">As for continuant fiat boundary, site, and spatial region</skos:example>
        <skos:prefLabel xml:lang="en">immaterial entity</skos:prefLabel>
    </owl:Class>
    


    <!-- http://purl.obolibrary.org/obo/BFO_0000142 -->

    <owl:Class rdf:about="http://purl.obolibrary.org/obo/BFO_0000142">
        <rdfs:subClassOf rdf:resource="http://purl.obolibrary.org/obo/BFO_0000140"/>
        <dc:identifier>032-BFO</dc:identifier>
        <rdfs:label xml:lang="en">fiat line</rdfs:label>
        <skos:definition xml:lang="en">(Elucidation) A fiat line is a continuant fiat boundary of one dimension that is continuous</skos:definition>
        <skos:example xml:lang="en">The Equator, all geopolitical boundaries, all lines of latitude and longitude, the median sulcus of your tongue, the line separating the outer surface of the mucosa of the lower lip from the outer surface of the skin of the chin</skos:example>
        <skos:prefLabel xml:lang="en">fiat line</skos:prefLabel>
    </owl:Class>
    


    <!-- http://purl.obolibrary.org/obo/BFO_0000145 -->

    <owl:Class rdf:about="http://purl.obolibrary.org/obo/BFO_0000145">
        <rdfs:subClassOf rdf:resource="http://purl.obolibrary.org/obo/BFO_0000019"/>
        <dc:identifier>057-BFO</dc:identifier>
        <rdfs:label xml:lang="en">relational quality</rdfs:label>
        <skos:definition xml:lang="en">b is a relational quality =Def b is a quality and there exists c and d such that c and d are not identical, b s-depends on c, and b s-depends on d</skos:definition>
        <skos:example xml:lang="en">A marriage bond, an instance of love, an obligation between one person and another</skos:example>
        <skos:prefLabel xml:lang="en">relational quality</skos:prefLabel>
    </owl:Class>
    


    <!-- http://purl.obolibrary.org/obo/BFO_0000146 -->

    <owl:Class rdf:about="http://purl.obolibrary.org/obo/BFO_0000146">
        <rdfs:subClassOf rdf:resource="http://purl.obolibrary.org/obo/BFO_0000140"/>
        <dc:identifier>033-BFO</dc:identifier>
        <rdfs:label xml:lang="en">fiat surface</rdfs:label>
        <skos:definition xml:lang="en">(Elucidation) A fiat surface is a continuant fiat boundary of two dimensions that is self-connected</skos:definition>
        <skos:example xml:lang="en">The surface of the Earth, the plane separating the smoking from the non-smoking zone in a restaurant</skos:example>
        <skos:prefLabel xml:lang="en">fiat surface</skos:prefLabel>
    </owl:Class>
    


    <!-- http://purl.obolibrary.org/obo/BFO_0000147 -->

    <owl:Class rdf:about="http://purl.obolibrary.org/obo/BFO_0000147">
        <rdfs:subClassOf rdf:resource="http://purl.obolibrary.org/obo/BFO_0000140"/>
        <dc:identifier>031-BFO</dc:identifier>
        <rdfs:label xml:lang="en">fiat point</rdfs:label>
        <skos:definition xml:lang="en">(Elucidation) A fiat point is a continuant fiat boundary of zero dimension that consists of a single point</skos:definition>
        <skos:example xml:lang="en">The geographic North Pole, the quadripoint where the boundaries of Colorado, Utah, New Mexico and Arizona meet, the point of origin of some spatial coordinate system</skos:example>
        <skos:prefLabel xml:lang="en">fiat point</skos:prefLabel>
    </owl:Class>
    


    <!-- http://purl.obolibrary.org/obo/BFO_0000148 -->

    <owl:Class rdf:about="http://purl.obolibrary.org/obo/BFO_0000148">
        <rdfs:subClassOf rdf:resource="http://purl.obolibrary.org/obo/BFO_0000008"/>
        <rdfs:subClassOf>
            <owl:Restriction>
                <owl:onProperty rdf:resource="http://purl.obolibrary.org/obo/BFO_0000121"/>
                <owl:allValuesFrom rdf:resource="http://purl.obolibrary.org/obo/BFO_0000148"/>
            </owl:Restriction>
        </rdfs:subClassOf>
        <dc:identifier>102-BFO</dc:identifier>
        <rdfs:label xml:lang="en">zero-dimensional temporal region</rdfs:label>
        <skos:definition xml:lang="en">(Elucidation) A zero-dimensional temporal region is a temporal region that is a whole consisting of one or more separated temporal instants as parts</skos:definition>
        <skos:example xml:lang="en">A temporal region that is occupied by a process boundary, the moment at which a finger is detached in an industrial accident</skos:example>
        <skos:prefLabel xml:lang="en">zero-dimensional temporal region</skos:prefLabel>
    </owl:Class>
    


    <!-- http://purl.obolibrary.org/obo/BFO_0000182 -->

    <owl:Class rdf:about="http://purl.obolibrary.org/obo/BFO_0000182">
        <rdfs:subClassOf rdf:resource="http://purl.obolibrary.org/obo/BFO_0000015"/>
        <dc:identifier>138-BFO</dc:identifier>
        <rdfs:label xml:lang="en">history</rdfs:label>
        <skos:definition xml:lang="en">(Elucidation) A history is a process that is the sum of the totality of processes taking place in the spatiotemporal region occupied by the material part of a material entity</skos:definition>
        <skos:example xml:lang="en">The life of an organism from the beginning to the end of its existence.</skos:example>
        <skos:prefLabel xml:lang="en">history</skos:prefLabel>
    </owl:Class>
    


    <!-- http://purl.obolibrary.org/obo/BFO_0000202 -->

    <owl:Class rdf:about="http://purl.obolibrary.org/obo/BFO_0000202">
        <rdfs:subClassOf rdf:resource="http://purl.obolibrary.org/obo/BFO_0000038"/>
        <dc:identifier>155-BFO</dc:identifier>
        <rdfs:label xml:lang="en">temporal interval</rdfs:label>
        <skos:definition xml:lang="en">(Elucidation) A temporal interval is a one-dimensional temporal region that is continuous, thus without gaps or breaks</skos:definition>
        <skos:example xml:lang="en">The year 2018</skos:example>
        <skos:prefLabel xml:lang="en">temporal interval</skos:prefLabel>
        <skos:scopeNote xml:lang="en">A one-dimensional temporal region can include as parts not only temporal intervals but also temporal instants separated from other parts by gaps</skos:scopeNote>
    </owl:Class>
    


    <!-- http://purl.obolibrary.org/obo/BFO_0000203 -->

    <owl:Class rdf:about="http://purl.obolibrary.org/obo/BFO_0000203">
        <rdfs:subClassOf rdf:resource="http://purl.obolibrary.org/obo/BFO_0000148"/>
        <dc:identifier>209-BFO</dc:identifier>
        <rdfs:label xml:lang="en">temporal instant</rdfs:label>
        <skos:definition xml:lang="en">(Elucidation) A temporal instant is a zero-dimensional temporal region that has no proper temporal part</skos:definition>
        <skos:example xml:lang="en">The millennium</skos:example>
        <skos:prefLabel xml:lang="en">temporal instant</skos:prefLabel>
    </owl:Class>
    


    <!-- 
    ///////////////////////////////////////////////////////////////////////////////////////
    //
    // General axioms
    //
    ///////////////////////////////////////////////////////////////////////////////////////
     -->

    <rdf:Description>
        <rdf:type rdf:resource="http://www.w3.org/2002/07/owl#AllDisjointClasses"/>
        <owl:members rdf:parseType="Collection">
            <rdf:Description rdf:about="http://purl.obolibrary.org/obo/BFO_0000004"/>
            <rdf:Description rdf:about="http://purl.obolibrary.org/obo/BFO_0000020"/>
            <rdf:Description rdf:about="http://purl.obolibrary.org/obo/BFO_0000031"/>
        </owl:members>
    </rdf:Description>
    <rdf:Description>
        <rdf:type rdf:resource="http://www.w3.org/2002/07/owl#AllDisjointClasses"/>
        <owl:members rdf:parseType="Collection">
            <rdf:Description rdf:about="http://purl.obolibrary.org/obo/BFO_0000006"/>
            <rdf:Description rdf:about="http://purl.obolibrary.org/obo/BFO_0000029"/>
            <rdf:Description rdf:about="http://purl.obolibrary.org/obo/BFO_0000140"/>
        </owl:members>
    </rdf:Description>
    <rdf:Description>
        <rdf:type rdf:resource="http://www.w3.org/2002/07/owl#AllDisjointClasses"/>
        <owl:members rdf:parseType="Collection">
            <rdf:Description rdf:about="http://purl.obolibrary.org/obo/BFO_0000008"/>
            <rdf:Description rdf:about="http://purl.obolibrary.org/obo/BFO_0000011"/>
            <rdf:Description rdf:about="http://purl.obolibrary.org/obo/BFO_0000015"/>
            <rdf:Description rdf:about="http://purl.obolibrary.org/obo/BFO_0000035"/>
        </owl:members>
    </rdf:Description>
    <rdf:Description>
        <rdf:type rdf:resource="http://www.w3.org/2002/07/owl#AllDisjointClasses"/>
        <owl:members rdf:parseType="Collection">
            <rdf:Description rdf:about="http://purl.obolibrary.org/obo/BFO_0000009"/>
            <rdf:Description rdf:about="http://purl.obolibrary.org/obo/BFO_0000018"/>
            <rdf:Description rdf:about="http://purl.obolibrary.org/obo/BFO_0000026"/>
            <rdf:Description rdf:about="http://purl.obolibrary.org/obo/BFO_0000028"/>
        </owl:members>
    </rdf:Description>
    <rdf:Description>
        <rdf:type rdf:resource="http://www.w3.org/2002/07/owl#AllDisjointClasses"/>
        <owl:members rdf:parseType="Collection">
            <rdf:Description rdf:about="http://purl.obolibrary.org/obo/BFO_0000142"/>
            <rdf:Description rdf:about="http://purl.obolibrary.org/obo/BFO_0000146"/>
            <rdf:Description rdf:about="http://purl.obolibrary.org/obo/BFO_0000147"/>
        </owl:members>
    </rdf:Description>
</rdf:RDF>
<!-- Generated by the OWL API (version 4.5.9.2019-02-01T07:24:44Z) https://github.com/owlcs/owlapi -->
